# baseURI: https://spec.edmcouncil.org/fibo/ontology/master/2025Q1/LOAN/LoansSpecific/CardAccounts/
# imports: https://spec.edmcouncil.org/fibo/ontology/master/2025Q1/FBC/DebtAndEquities/Debt/
# imports: https://spec.edmcouncil.org/fibo/ontology/master/2025Q1/FBC/FinancialInstruments/FinancialInstruments/
# imports: https://spec.edmcouncil.org/fibo/ontology/master/2025Q1/FBC/ProductsAndServices/ClientsAndAccounts/
# imports: https://spec.edmcouncil.org/fibo/ontology/master/2025Q1/FBC/ProductsAndServices/FinancialProductsAndServices/
# imports: https://spec.edmcouncil.org/fibo/ontology/master/2025Q1/FND/Accounting/CurrencyAmount/
# imports: https://spec.edmcouncil.org/fibo/ontology/master/2025Q1/FND/Agreements/Contracts/
# imports: https://spec.edmcouncil.org/fibo/ontology/master/2025Q1/FND/Arrangements/Documents/
# imports: https://spec.edmcouncil.org/fibo/ontology/master/2025Q1/FND/OwnershipAndControl/Ownership/
# imports: https://spec.edmcouncil.org/fibo/ontology/master/2025Q1/FND/ProductsAndServices/ProductsAndServices/
# imports: https://spec.edmcouncil.org/fibo/ontology/master/2025Q1/FND/Relations/Relations/
# imports: https://spec.edmcouncil.org/fibo/ontology/master/2025Q1/FND/Utilities/AnnotationVocabulary/
# imports: https://spec.edmcouncil.org/fibo/ontology/master/2025Q1/LOAN/LoansSpecific/ConsumerLoans/
# imports: https://www.omg.org/spec/Commons/AnnotationVocabulary/
# imports: https://www.omg.org/spec/Commons/Classifiers/
# imports: https://www.omg.org/spec/Commons/CodesAndCodeSets/
# imports: https://www.omg.org/spec/Commons/ContextualDesignators/
# imports: https://www.omg.org/spec/Commons/DatesAndTimes/
# imports: https://www.omg.org/spec/Commons/Designators/
# imports: https://www.omg.org/spec/Commons/Identifiers/
# imports: https://www.omg.org/spec/Commons/Locations/
# imports: https://www.omg.org/spec/Commons/Organizations/
# imports: https://www.omg.org/spec/Commons/PartiesAndSituations/
# imports: https://www.omg.org/spec/Commons/RolesAndCompositions/

@base <https://spec.edmcouncil.org/fibo/ontology/master/2025Q1/LOAN/LoansSpecific/CardAccounts/> .
@prefix cmns-av: <https://www.omg.org/spec/Commons/AnnotationVocabulary/> .
@prefix cmns-cds: <https://www.omg.org/spec/Commons/CodesAndCodeSets/> .
@prefix cmns-cls: <https://www.omg.org/spec/Commons/Classifiers/> .
@prefix cmns-cxtdsg: <https://www.omg.org/spec/Commons/ContextualDesignators/> .
@prefix cmns-doc: <https://www.omg.org/spec/Commons/Documents/> .
@prefix cmns-dsg: <https://www.omg.org/spec/Commons/Designators/> .
@prefix cmns-dt: <https://www.omg.org/spec/Commons/DatesAndTimes/> .
@prefix cmns-id: <https://www.omg.org/spec/Commons/Identifiers/> .
@prefix cmns-loc: <https://www.omg.org/spec/Commons/Locations/> .
@prefix cmns-org: <https://www.omg.org/spec/Commons/Organizations/> .
@prefix cmns-pts: <https://www.omg.org/spec/Commons/PartiesAndSituations/> .
@prefix cmns-rlcmp: <https://www.omg.org/spec/Commons/RolesAndCompositions/> .
@prefix dcterms: <http://purl.org/dc/terms/> .
@prefix fibo-fbc-dae-dbt: <https://spec.edmcouncil.org/fibo/ontology/FBC/DebtAndEquities/Debt/> .
@prefix fibo-fbc-fi-fi: <https://spec.edmcouncil.org/fibo/ontology/FBC/FinancialInstruments/FinancialInstruments/> .
@prefix fibo-fbc-pas-caa: <https://spec.edmcouncil.org/fibo/ontology/FBC/ProductsAndServices/ClientsAndAccounts/> .
@prefix fibo-fbc-pas-fpas: <https://spec.edmcouncil.org/fibo/ontology/FBC/ProductsAndServices/FinancialProductsAndServices/> .
@prefix fibo-fnd-acc-cur: <https://spec.edmcouncil.org/fibo/ontology/FND/Accounting/CurrencyAmount/> .
@prefix fibo-fnd-agr-ctr: <https://spec.edmcouncil.org/fibo/ontology/FND/Agreements/Contracts/> .
@prefix fibo-fnd-arr-doc: <https://spec.edmcouncil.org/fibo/ontology/FND/Arrangements/Documents/> .
@prefix fibo-fnd-oac-own: <https://spec.edmcouncil.org/fibo/ontology/FND/OwnershipAndControl/Ownership/> .
@prefix fibo-fnd-pas-pas: <https://spec.edmcouncil.org/fibo/ontology/FND/ProductsAndServices/ProductsAndServices/> .
@prefix fibo-fnd-rel-rel: <https://spec.edmcouncil.org/fibo/ontology/FND/Relations/Relations/> .
@prefix fibo-fnd-utl-av: <https://spec.edmcouncil.org/fibo/ontology/FND/Utilities/AnnotationVocabulary/> .
@prefix fibo-loan-spc-cns: <https://spec.edmcouncil.org/fibo/ontology/LOAN/LoansSpecific/ConsumerLoans/> .
@prefix fibo-loan-spc-crd: <https://spec.edmcouncil.org/fibo/ontology/LOAN/LoansSpecific/CardAccounts/> .
@prefix owl: <http://www.w3.org/2002/07/owl#> .
@prefix rdf: <http://www.w3.org/1999/02/22-rdf-syntax-ns#> .
@prefix rdfs: <http://www.w3.org/2000/01/rdf-schema#> .
@prefix skos: <http://www.w3.org/2004/02/skos/core#> .
@prefix xsd: <http://www.w3.org/2001/XMLSchema#> .

<https://spec.edmcouncil.org/fibo/ontology/LOAN/LoansSpecific/CardAccounts/>
	a owl:Ontology ;
	rdfs:label "Card Accounts Ontology" ;
	dcterms:abstract "This ontology defines revolving credit account-related concepts that are specific to credit and debit cards. Note that it does not differentiate between consumer and commercial/corporate cards and is capable of representing either." ;
	dcterms:license """Copyright (c) 2020-2025 EDM Council, Inc.
		Copyright (c) 2020-2025 Object Management Group, Inc.
		
		Permission is hereby granted, free of charge, to any person obtaining a copy of this software and associated documentation files (the 'Software'), to deal in the Software without restriction, including without limitation the rights to use, copy, modify, merge, publish, distribute, sublicense, and/or sell copies of the Software, and to permit persons to whom the Software is furnished to do so, subject to the following conditions:

The above copyright notice and this permission notice shall be included in all copies or substantial portions of the Software.

THE SOFTWARE IS PROVIDED 'AS IS', WITHOUT WARRANTY OF ANY KIND, EXPRESS OR IMPLIED, INCLUDING BUT NOT LIMITED TO THE WARRANTIES OF MERCHANTABILITY, FITNESS FOR A PARTICULAR PURPOSE AND NONINFRINGEMENT. IN NO EVENT SHALL THE AUTHORS OR COPYRIGHT HOLDERS BE LIABLE FOR ANY CLAIM, DAMAGES OR OTHER LIABILITY, WHETHER IN AN ACTION OF CONTRACT, TORT OR OTHERWISE, ARISING FROM, OUT OF OR IN CONNECTION WITH THE SOFTWARE OR THE USE OR OTHER DEALINGS IN THE SOFTWARE.
		
		See https://opensource.org/licenses/MIT.""" ;
	owl:imports
		<https://spec.edmcouncil.org/fibo/ontology/master/2025Q1/FBC/DebtAndEquities/Debt/> ,
		<https://spec.edmcouncil.org/fibo/ontology/master/2025Q1/FBC/FinancialInstruments/FinancialInstruments/> ,
		<https://spec.edmcouncil.org/fibo/ontology/master/2025Q1/FBC/ProductsAndServices/ClientsAndAccounts/> ,
		<https://spec.edmcouncil.org/fibo/ontology/master/2025Q1/FBC/ProductsAndServices/FinancialProductsAndServices/> ,
		<https://spec.edmcouncil.org/fibo/ontology/master/2025Q1/FND/Accounting/CurrencyAmount/> ,
		<https://spec.edmcouncil.org/fibo/ontology/master/2025Q1/FND/Agreements/Contracts/> ,
		<https://spec.edmcouncil.org/fibo/ontology/master/2025Q1/FND/Arrangements/Documents/> ,
		<https://spec.edmcouncil.org/fibo/ontology/master/2025Q1/FND/OwnershipAndControl/Ownership/> ,
		<https://spec.edmcouncil.org/fibo/ontology/master/2025Q1/FND/ProductsAndServices/ProductsAndServices/> ,
		<https://spec.edmcouncil.org/fibo/ontology/master/2025Q1/FND/Relations/Relations/> ,
		<https://spec.edmcouncil.org/fibo/ontology/master/2025Q1/FND/Utilities/AnnotationVocabulary/> ,
		<https://spec.edmcouncil.org/fibo/ontology/master/2025Q1/LOAN/LoansSpecific/ConsumerLoans/> ,
		<https://www.omg.org/spec/Commons/AnnotationVocabulary/> ,
		<https://www.omg.org/spec/Commons/Classifiers/> ,
		<https://www.omg.org/spec/Commons/CodesAndCodeSets/> ,
		<https://www.omg.org/spec/Commons/ContextualDesignators/> ,
		<https://www.omg.org/spec/Commons/DatesAndTimes/> ,
		<https://www.omg.org/spec/Commons/Designators/> ,
		<https://www.omg.org/spec/Commons/Identifiers/> ,
		<https://www.omg.org/spec/Commons/Locations/> ,
		<https://www.omg.org/spec/Commons/Organizations/> ,
		<https://www.omg.org/spec/Commons/PartiesAndSituations/> ,
		<https://www.omg.org/spec/Commons/RolesAndCompositions/>
		;
	owl:versionIRI <https://spec.edmcouncil.org/fibo/ontology/master/2025Q1/LOAN/LoansSpecific/CardAccounts/> ;
	skos:changeNote
		"The https://spec.edmcouncil.org/fibo/ontology/LOAN/LoansSpecific/CardAccounts.rdf version of the ontology was modified to improve the class hierarchy for credit card agreement." ,
		"The https://spec.edmcouncil.org/fibo/ontology/LOAN/LoansSpecific/CardAccounts.rdf version of the ontology was modified to replace additional concepts from several FIBO FND ontologies with their counterparts added to the Commons Ontology Library (Commons) v1.1." ,
		"The https://spec.edmcouncil.org/fibo/ontology/LOAN/LoansSpecific/CardAccounts.rdf version of the ontology was modified to replace additional content that is now available in the OMG Commons Ontology Library (Commons) v1.2 (FND-389)." ,
		"The https://spec.edmcouncil.org/fibo/ontology/LOAN/LoansSpecific/CardAccounts.rdf version of the ontology was modified to replace concepts from several FIBO FND ontologies with their counterparts added to the Commons Ontology Library (Commons) v1.1." ,
		"The https://spec.edmcouncil.org/fibo/ontology/LOAN/LoansSpecific/CardAccounts.rdf version of this ontology was modified to add a distinction between consumer and commercial credit card agreements." ,
		"The https://spec.edmcouncil.org/fibo/ontology/LOAN/LoansSpecific/CardAccounts.rdf version of this ontology was modified to make consumer credit card agreement a subclass of unsecured consumer loan."
		;
	fibo-fnd-utl-av:hasMaturityLevel fibo-fnd-utl-av:Release ;
	cmns-av:copyright
		"Copyright (c) 2020-2025 EDM Council, Inc." ,
		"Copyright (c) 2020-2025 Object Management Group, Inc."
		;
	.

fibo-loan-spc-crd:AmericanExpressNetwork
	a
		owl:NamedIndividual ,
		fibo-loan-spc-crd:CreditCardNetwork
		;
	rdfs:label "American Express network" ;
	rdfs:isDefinedBy <https://spec.edmcouncil.org/fibo/ontology/LOAN/LoansSpecific/CardAccounts/> ;
	skos:definition "credit card network and card issuer that both issues credit cards and processes payments for cards bearing its logo, as well as offering cardholder benefits like travel insurance" ;
	.

fibo-loan-spc-crd:CardAccount
	a owl:Class ;
	rdfs:subClassOf
		fibo-fbc-pas-caa:CustomerAccount ,
		[
			a owl:Restriction ;
			owl:onProperty fibo-fbc-pas-caa:isLinkedToAccount ;
			owl:onClass fibo-fbc-pas-caa:CustomerAccount ;
			owl:minQualifiedCardinality "0"^^xsd:nonNegativeInteger ;
		] ,
		[
			a owl:Restriction ;
			owl:onProperty fibo-fbc-pas-caa:hasPrimaryAccountHolder ;
			owl:someValuesFrom fibo-loan-spc-crd:Cardholder ;
		] ,
		[
			a owl:Restriction ;
			owl:onProperty fibo-fnd-rel-rel:exemplifies ;
			owl:someValuesFrom fibo-loan-spc-crd:CardProduct ;
		] ,
		[
			a owl:Restriction ;
			owl:onProperty cmns-dsg:isDefinedIn ;
			owl:someValuesFrom fibo-loan-spc-crd:PaymentCardAgreement ;
		] ,
		[
			a owl:Restriction ;
			owl:onProperty cmns-dsg:isSignifiedBy ;
			owl:someValuesFrom fibo-loan-spc-crd:PaymentCard ;
		] ,
		[
			a owl:Restriction ;
			owl:onProperty cmns-id:isIdentifiedBy ;
			owl:someValuesFrom fibo-loan-spc-crd:PrimaryCardAccountNumber ;
		]
		;
	rdfs:label "card account" ;
	rdfs:isDefinedBy <https://spec.edmcouncil.org/fibo/ontology/LOAN/LoansSpecific/CardAccounts/> ;
	skos:definition "account whose terms and conditions are defined in a card agreement that is represented by a payment card" ;
	.

fibo-loan-spc-crd:CardAuthenticationValue
	a owl:Class ;
	rdfs:subClassOf fibo-loan-spc-crd:MagneticStripeVerificationCodeValue ;
	rdfs:label "card authentication value" ;
	rdfs:isDefinedBy <https://spec.edmcouncil.org/fibo/ontology/LOAN/LoansSpecific/CardAccounts/> ;
	skos:definition "card verification value specifically for JCB payment cards" ;
	cmns-av:abbreviation "CAV" ;
	cmns-av:adaptedFrom "https://www.pcisecuritystandards.org/pci_security/glossary"^^xsd:anyURI ;
	.

fibo-loan-spc-crd:CardAuthenticationValue2
	a owl:Class ;
	rdfs:subClassOf fibo-loan-spc-crd:ThreeDigitVerificationCodeValue ;
	rdfs:label "card authentication value 2" ;
	rdfs:isDefinedBy <https://spec.edmcouncil.org/fibo/ontology/LOAN/LoansSpecific/CardAccounts/> ;
	skos:definition "card verification value specifically for JCB payment cards" ;
	cmns-av:adaptedFrom "https://www.pcisecuritystandards.org/pci_security/glossary"^^xsd:anyURI ;
	cmns-av:synonym "CAV2" ;
	.

fibo-loan-spc-crd:CardExpirationDate
	a owl:Class ;
	rdfs:subClassOf cmns-dt:ExplicitDate ;
	rdfs:label "card expiration date" ;
	rdfs:isDefinedBy <https://spec.edmcouncil.org/fibo/ontology/LOAN/LoansSpecific/CardAccounts/> ;
	skos:definition "date on which a given payment card expires" ;
	.

fibo-loan-spc-crd:CardIdentificationNumber
	a owl:Class ;
	rdfs:subClassOf fibo-loan-spc-crd:ThreeDigitVerificationCodeValue ;
	rdfs:label "card identification number" ;
	rdfs:isDefinedBy <https://spec.edmcouncil.org/fibo/ontology/LOAN/LoansSpecific/CardAccounts/> ;
	skos:definition "card verification value specifically for American Express and Discover payment cards" ;
	cmns-av:abbreviation "CID" ;
	cmns-av:adaptedFrom "https://www.pcisecuritystandards.org/pci_security/glossary"^^xsd:anyURI ;
	.

fibo-loan-spc-crd:CardProduct
	a owl:Class ;
	rdfs:subClassOf
		fibo-fbc-pas-fpas:FinancialProduct ,
		[
			a owl:Restriction ;
			owl:onProperty fibo-loan-spc-crd:hasCreditCardNetwork ;
			owl:onClass fibo-loan-spc-crd:CreditCardNetwork ;
			owl:minQualifiedCardinality "0"^^xsd:nonNegativeInteger ;
		] ,
		[
			a owl:Restriction ;
			owl:onProperty cmns-loc:hasSubdivision ;
			owl:onClass cmns-loc:CountrySubdivision ;
			owl:minQualifiedCardinality "0"^^xsd:nonNegativeInteger ;
		] ,
		[
			a owl:Restriction ;
			owl:onProperty fibo-loan-spc-crd:usesCurrency ;
			owl:onClass fibo-fnd-acc-cur:Currency ;
			owl:qualifiedCardinality "1"^^xsd:nonNegativeInteger ;
		] ,
		[
			a owl:Restriction ;
			owl:onProperty cmns-loc:hasCountry ;
			owl:onClass cmns-loc:Country ;
			owl:qualifiedCardinality "1"^^xsd:nonNegativeInteger ;
		] ,
		[
			a owl:Restriction ;
			owl:onProperty fibo-fnd-rel-rel:isExemplifiedBy ;
			owl:someValuesFrom fibo-loan-spc-crd:CardAccount ;
		]
		;
	rdfs:label "card product" ;
	rdfs:isDefinedBy <https://spec.edmcouncil.org/fibo/ontology/LOAN/LoansSpecific/CardAccounts/> ;
	skos:definition "financial product involving the issuance of credit, debit, or other payment cards" ;
	.

fibo-loan-spc-crd:CardSecurityCode
	a owl:Class ;
	rdfs:subClassOf fibo-loan-spc-crd:MagneticStripeVerificationCodeValue ;
	rdfs:label "card security code" ;
	rdfs:isDefinedBy <https://spec.edmcouncil.org/fibo/ontology/LOAN/LoansSpecific/CardAccounts/> ;
	skos:definition "card verification value specifically for American Express payment cards" ;
	cmns-av:abbreviation "CSC" ;
	cmns-av:adaptedFrom "https://www.pcisecuritystandards.org/pci_security/glossary"^^xsd:anyURI ;
	.

fibo-loan-spc-crd:CardValidationCode
	a owl:Class ;
	rdfs:subClassOf fibo-loan-spc-crd:MagneticStripeVerificationCodeValue ;
	rdfs:label "card validation code" ;
	rdfs:isDefinedBy <https://spec.edmcouncil.org/fibo/ontology/LOAN/LoansSpecific/CardAccounts/> ;
	skos:definition "card verification code specifically for Mastercard payment cards" ;
	cmns-av:abbreviation "PAN CVC" ;
	cmns-av:adaptedFrom "https://www.pcisecuritystandards.org/pci_security/glossary"^^xsd:anyURI ;
	.

fibo-loan-spc-crd:CardValidationCode2
	a owl:Class ;
	rdfs:subClassOf fibo-loan-spc-crd:ThreeDigitVerificationCodeValue ;
	rdfs:label "card validation code 2" ;
	rdfs:isDefinedBy <https://spec.edmcouncil.org/fibo/ontology/LOAN/LoansSpecific/CardAccounts/> ;
	skos:definition "card verification value specifically for Mastercard payment cards" ;
	cmns-av:abbreviation "PAN CVC2" ;
	cmns-av:adaptedFrom "https://www.pcisecuritystandards.org/pci_security/glossary"^^xsd:anyURI ;
	.

fibo-loan-spc-crd:CardVerificationCodeValue
	a owl:Class ;
	rdfs:subClassOf
		cmns-cds:CodeElement ,
		[
			a owl:Restriction ;
			owl:onProperty fibo-fnd-rel-rel:hasTag ;
			owl:onDataRange xsd:string ;
			owl:qualifiedCardinality "1"^^xsd:nonNegativeInteger ;
		] ,
		[
			a owl:Restriction ;
			owl:onProperty cmns-cxtdsg:appliesTo ;
			owl:someValuesFrom fibo-loan-spc-crd:PaymentCard ;
		]
		;
	rdfs:label "card verification code or value" ;
	rdfs:isDefinedBy <https://spec.edmcouncil.org/fibo/ontology/LOAN/LoansSpecific/CardAccounts/> ;
	skos:definition "code that specifies either (1) magnetic-stripe data, or (2) printed security features that are used to protect data integrity and limit alteration, counterfeiting and fraud generally" ;
	cmns-av:adaptedFrom "https://www.pcisecuritystandards.org/pci_security/glossary"^^xsd:anyURI ;
	.

fibo-loan-spc-crd:CardVerificationValue
	a owl:Class ;
	rdfs:subClassOf fibo-loan-spc-crd:MagneticStripeVerificationCodeValue ;
	rdfs:label "card verification value" ;
	rdfs:isDefinedBy <https://spec.edmcouncil.org/fibo/ontology/LOAN/LoansSpecific/CardAccounts/> ;
	skos:definition "card verification value specifically for Visa and Discover payment cards" ;
	cmns-av:abbreviation "CVV" ;
	cmns-av:adaptedFrom "https://www.pcisecuritystandards.org/pci_security/glossary"^^xsd:anyURI ;
	.

fibo-loan-spc-crd:CardVerificationValue2
	a owl:Class ;
	rdfs:subClassOf fibo-loan-spc-crd:ThreeDigitVerificationCodeValue ;
	rdfs:label "card verification value 2" ;
	rdfs:isDefinedBy <https://spec.edmcouncil.org/fibo/ontology/LOAN/LoansSpecific/CardAccounts/> ;
	skos:definition "card verification value specifically for Visa payment cards" ;
	cmns-av:adaptedFrom "https://www.pcisecuritystandards.org/pci_security/glossary"^^xsd:anyURI ;
	cmns-av:synonym "CVV2" ;
	.

fibo-loan-spc-crd:Cardholder
	a owl:Class ;
	rdfs:subClassOf
		fibo-fbc-pas-caa:CustomerAccountHolder ,
		[
			a owl:Restriction ;
			owl:onProperty fibo-fnd-rel-rel:holds ;
			owl:someValuesFrom fibo-loan-spc-crd:CardAccount ;
		] ,
		[
			a owl:Restriction ;
			owl:onProperty cmns-rlcmp:isPlayedBy ;
			owl:someValuesFrom [
				a owl:Restriction ;
				owl:onProperty fibo-fnd-oac-own:owns ;
				owl:someValuesFrom fibo-loan-spc-crd:CardAccount ;
			] ;
		] ,
		[
			a owl:Restriction ;
			owl:onProperty cmns-rlcmp:isPlayedBy ;
			owl:someValuesFrom [
				a owl:Restriction ;
				owl:onProperty cmns-pts:isAPartyTo ;
				owl:someValuesFrom fibo-loan-spc-crd:CardAccount ;
			] ;
		]
		;
	rdfs:label "cardholder" ;
	rdfs:isDefinedBy <https://spec.edmcouncil.org/fibo/ontology/LOAN/LoansSpecific/CardAccounts/> ;
	skos:definition "account holder to whom a payment card is issued" ;
	cmns-av:adaptedFrom "https://www.pcisecuritystandards.org/pci_security/glossary"^^xsd:anyURI ;
	.

fibo-loan-spc-crd:CommercialCreditCardAgreement
	a owl:Class ;
	rdfs:subClassOf
		fibo-loan-spc-crd:CreditCardAgreement ,
		[
			a owl:Restriction ;
			owl:onProperty fibo-fbc-dae-dbt:hasBorrower ;
			owl:someValuesFrom [
				a owl:Restriction ;
				owl:onProperty cmns-rlcmp:isPlayedBy ;
				owl:someValuesFrom cmns-org:FormalOrganization ;
			] ;
		]
		;
	rdfs:label "commercial credit card agreement" ;
	rdfs:isDefinedBy <https://spec.edmcouncil.org/fibo/ontology/LOAN/LoansSpecific/CardAccounts/> ;
	skos:definition "credit card agreement for a card issued to, or in conjunction with, a formal organization, such as a small business, middle market business, local, state, or national government, or large corporation" ;
	cmns-av:adaptedFrom "https://www.fdic.gov/regulations/examinations/credit_card/pdf_version/ch2.pdf"^^xsd:anyURI ;
	cmns-av:explanatoryNote "Corporate card programs come in more than one form to serve different business needs. In general, they are contractual agreements between a sponsoring entity and a financial institution, in which the financial institution issues corporate cards to select employees of the sponsoring company." ;
	cmns-av:synonym "corporate credit card agreement" ;
	.

fibo-loan-spc-crd:ConsumerCreditCardAgreement
	a owl:Class ;
	rdfs:subClassOf
		fibo-loan-spc-crd:CreditCardAgreement ,
		fibo-loan-spc-cns:UnsecuredConsumerLoan ,
		[
			a owl:Restriction ;
			owl:onProperty fibo-fbc-dae-dbt:hasBorrower ;
			owl:someValuesFrom fibo-fnd-pas-pas:Consumer ;
		]
		;
	rdfs:label "consumer credit card agreement" ;
	rdfs:isDefinedBy <https://spec.edmcouncil.org/fibo/ontology/LOAN/LoansSpecific/CardAccounts/> ;
	skos:definition "credit card agreement for a card issued for household, family, or other personal expenditures that is accessed by a borrower's use of a credit card" ;
	cmns-av:adaptedFrom "https://www.law.cornell.edu/cfr/text/12/228.12"^^xsd:anyURI ;
	.

fibo-loan-spc-crd:CreditCard
	a owl:Class ;
	rdfs:subClassOf
		fibo-loan-spc-crd:PaymentCard ,
		[
			a owl:Restriction ;
			owl:onProperty fibo-fnd-agr-ctr:isEvidenceFor ;
			owl:onClass fibo-loan-spc-crd:CreditCardAccount ;
			owl:qualifiedCardinality "1"^^xsd:nonNegativeInteger ;
		] ,
		[
			a owl:Restriction ;
			owl:onProperty cmns-cls:isClassifiedBy ;
			owl:someValuesFrom fibo-loan-spc-crd:CreditCardProduct ;
		]
		;
	rdfs:label "credit card" ;
	rdfs:isDefinedBy <https://spec.edmcouncil.org/fibo/ontology/LOAN/LoansSpecific/CardAccounts/> ;
	skos:definition "card issued by a financial service provider that enables the cardholder to borrow funds" ;
	cmns-av:adaptedFrom "https://www.fdic.gov/regulations/examinations/credit_card/pdf_version/ch2.pdf"^^xsd:anyURI ;
	cmns-av:explanatoryNote
		"In its non-physical form, a credit card represents a payment mechanism which facilitates both consumer and commercial business transactions, including purchases and cash advances. A credit card generally operates as a substitute for cash or a check and most often provides an unsecured revolving line of credit. The borrower is required to pay at least part of the card's outstanding balance each billing cycle, depending on the terms as set forth in the cardholder agreement. As the debt reduces, the available credit increases for accounts in good standing. These complex financial arrangements have ever-shifting terms and prices. A charge card differs from a credit card in that the charge card must be paid in full each month." ,
		"In physical form, a credit card traditionally is a thin, rectangular plastic card. The front of the card contains a series of numbers that are representative of various items such as the applicable network, bank, and account." ,
		"Issuance of credit cards has the condition that the cardholder will pay back the original, borrowed amount plus any additional agreed-upon charges. The credit company provider may also grant a line of credit (LOC) to the cardholder which allows the holder to borrow money in the form of a cash advance. The issuer pre-sets borrowing limits which have a basis on the individual's credit rating."
		;
	.

fibo-loan-spc-crd:CreditCardAccount
	a owl:Class ;
	rdfs:subClassOf
		fibo-fbc-pas-caa:LoanOrCreditAccount ,
		fibo-loan-spc-crd:CardAccount ,
		[
			a owl:Restriction ;
			owl:onProperty fibo-fbc-pas-caa:hasPaymentDueDate ;
			owl:someValuesFrom fibo-fbc-pas-caa:PaymentDueDate ;
		] ,
		[
			a owl:Restriction ;
			owl:onProperty fibo-fnd-rel-rel:exemplifies ;
			owl:someValuesFrom fibo-loan-spc-crd:CreditCardProduct ;
		] ,
		[
			a owl:Restriction ;
			owl:onProperty cmns-dsg:isDefinedIn ;
			owl:someValuesFrom fibo-loan-spc-crd:CreditCardAgreement ;
		] ,
		[
			a owl:Restriction ;
			owl:onProperty cmns-dsg:isSignifiedBy ;
			owl:someValuesFrom fibo-loan-spc-crd:CreditCard ;
		]
		;
	rdfs:label "credit card account" ;
	rdfs:isDefinedBy <https://spec.edmcouncil.org/fibo/ontology/LOAN/LoansSpecific/CardAccounts/> ;
	skos:definition "card account whose terms and conditions are defined in a credit card agreement that is represented by a credit card" ;
	.

fibo-loan-spc-crd:CreditCardAgreement
	a owl:Class ;
	rdfs:subClassOf
		fibo-fbc-dae-dbt:CommittedCreditFacility ,
		fibo-loan-spc-crd:PaymentCardAgreement ,
		[
			a owl:Restriction ;
			owl:onProperty fibo-fbc-dae-dbt:hasBorrower ;
			owl:someValuesFrom fibo-loan-spc-crd:Cardholder ;
		] ,
		[
			a owl:Restriction ;
			owl:onProperty fibo-fbc-dae-dbt:hasLender ;
			owl:someValuesFrom fibo-loan-spc-crd:IssuingFinancialInstitution ;
		] ,
		[
			a owl:Restriction ;
			owl:onProperty fibo-fnd-agr-ctr:isEvidencedBy ;
			owl:someValuesFrom fibo-loan-spc-crd:CreditCard ;
		] ,
		[
			a owl:Restriction ;
			owl:onProperty cmns-cxtdsg:appliesTo ;
			owl:someValuesFrom fibo-loan-spc-crd:CreditCardAccount ;
		]
		;
	rdfs:label "credit card agreement" ;
	rdfs:isDefinedBy <https://spec.edmcouncil.org/fibo/ontology/LOAN/LoansSpecific/CardAccounts/> ;
	skos:definition "account-specific credit facility that specifies the terms and conditions under which the credit card is offered to the cardholder by the issuer" ;
	.

fibo-loan-spc-crd:CreditCardNetwork
	a owl:Class ;
	rdfs:subClassOf
		cmns-cls:Classifier ,
		[
			a owl:Restriction ;
			owl:onProperty fibo-fnd-rel-rel:hasTag ;
			owl:someValuesFrom xsd:string ;
		] ,
		[
			a owl:Restriction ;
			owl:onProperty cmns-cls:classifies ;
			owl:someValuesFrom fibo-loan-spc-crd:CardProduct ;
		]
		;
	rdfs:label "credit card network" ;
	rdfs:isDefinedBy <https://spec.edmcouncil.org/fibo/ontology/LOAN/LoansSpecific/CardAccounts/> ;
	skos:definition "classifier for the network that authorizes, processes, and sets the terms of credit card transactions, as well as transfers payments between shoppers, merchants, and their banks" ;
	skos:example "Mastercard, Visa, American Express, Discover" ;
	.

fibo-loan-spc-crd:CreditCardProduct
	a owl:Class ;
	rdfs:subClassOf
		fibo-loan-spc-crd:CardProduct ,
		[
			a owl:Restriction ;
			owl:onProperty fibo-loan-spc-crd:hasCreditCardNetwork ;
			owl:onClass fibo-loan-spc-crd:CreditCardNetwork ;
			owl:qualifiedCardinality "1"^^xsd:nonNegativeInteger ;
		] ,
		[
			a owl:Restriction ;
			owl:onProperty fibo-fnd-rel-rel:isExemplifiedBy ;
			owl:someValuesFrom fibo-loan-spc-crd:CreditCardAccount ;
		] ,
		[
			a owl:Restriction ;
			owl:onProperty cmns-cls:classifies ;
			owl:someValuesFrom fibo-loan-spc-crd:CreditCard ;
		]
		;
	rdfs:label "credit card product" ;
	rdfs:isDefinedBy <https://spec.edmcouncil.org/fibo/ontology/LOAN/LoansSpecific/CardAccounts/> ;
	skos:definition "card product allowing the holder to purchase goods or services on credit" ;
	.

fibo-loan-spc-crd:DebitCard
	a owl:Class ;
	rdfs:subClassOf
		fibo-loan-spc-crd:PaymentCard ,
		[
			a owl:Restriction ;
			owl:onProperty fibo-fnd-agr-ctr:isEvidenceFor ;
			owl:onClass fibo-loan-spc-crd:DebitCardAccount ;
			owl:qualifiedCardinality "1"^^xsd:nonNegativeInteger ;
		] ,
		[
			a owl:Restriction ;
			owl:onProperty cmns-cls:isClassifiedBy ;
			owl:someValuesFrom fibo-loan-spc-crd:DebitCardProduct ;
		]
		;
	rdfs:label "debit card" ;
	rdfs:isDefinedBy <https://spec.edmcouncil.org/fibo/ontology/LOAN/LoansSpecific/CardAccounts/> ;
	skos:definition "payment card issued by a financial service provider that enables the cardholder to access funds in a demand deposit account" ;
	.

fibo-loan-spc-crd:DebitCardAccount
	a owl:Class ;
	rdfs:subClassOf
		fibo-loan-spc-crd:CardAccount ,
		[
			a owl:Restriction ;
			owl:onProperty fibo-fnd-rel-rel:exemplifies ;
			owl:someValuesFrom fibo-loan-spc-crd:DebitCardProduct ;
		] ,
		[
			a owl:Restriction ;
			owl:onProperty cmns-dsg:isSignifiedBy ;
			owl:someValuesFrom fibo-loan-spc-crd:DebitCard ;
		]
		;
	rdfs:label "debit card account" ;
	rdfs:isDefinedBy <https://spec.edmcouncil.org/fibo/ontology/LOAN/LoansSpecific/CardAccounts/> ;
	skos:definition "card account that is represented by a one or more debit cards" ;
	.

fibo-loan-spc-crd:DebitCardProduct
	a owl:Class ;
	rdfs:subClassOf
		fibo-loan-spc-crd:CardProduct ,
		[
			a owl:Restriction ;
			owl:onProperty fibo-fnd-rel-rel:isExemplifiedBy ;
			owl:someValuesFrom fibo-loan-spc-crd:DebitCardAccount ;
		] ,
		[
			a owl:Restriction ;
			owl:onProperty cmns-cls:classifies ;
			owl:someValuesFrom fibo-loan-spc-crd:DebitCard ;
		]
		;
	rdfs:label "debit card product" ;
	rdfs:isDefinedBy <https://spec.edmcouncil.org/fibo/ontology/LOAN/LoansSpecific/CardAccounts/> ;
	skos:definition "card product card typically provided by a depository institution allowing the holder to transfer money electronically to another account when making a purchase" ;
	.

fibo-loan-spc-crd:DiscoverNetwork
	a
		owl:NamedIndividual ,
		fibo-loan-spc-crd:CreditCardNetwork
		;
	rdfs:label "Discover network" ;
	rdfs:isDefinedBy <https://spec.edmcouncil.org/fibo/ontology/LOAN/LoansSpecific/CardAccounts/> ;
	skos:definition "credit card network and card issuer offering benefits like secondary rental car collision insurance" ;
	.

fibo-loan-spc-crd:IssuingFinancialInstitution
	a owl:Class ;
	rdfs:subClassOf
		fibo-fbc-fi-fi:Issuer ,
		fibo-fbc-pas-fpas:FinancialServiceProvider
		;
	rdfs:label "issuing financial institution" ;
	rdfs:isDefinedBy <https://spec.edmcouncil.org/fibo/ontology/LOAN/LoansSpecific/CardAccounts/> ;
	skos:definition "issuer and financial services provider that issues payment cards or performs, facilitates, or supports issuing services including but not limited to issuing banks and issuing processors" ;
	cmns-av:adaptedFrom "https://www.pcisecuritystandards.org/pci_security/glossary"^^xsd:anyURI ;
	cmns-av:synonym "issuing bank" ;
	.

fibo-loan-spc-crd:JCBNetwork
	a
		owl:NamedIndividual ,
		fibo-loan-spc-crd:CreditCardNetwork
		;
	rdfs:label "JCB network" ;
	rdfs:isDefinedBy <https://spec.edmcouncil.org/fibo/ontology/LOAN/LoansSpecific/CardAccounts/> ;
	skos:definition "credit card network based in Japan, with coverage throughout Asia, with strategic partners worldwide" ;
	cmns-av:explanatoryNote "JCB Co., Ltd., (formerly Japan Credit Bureau) is a credit card company based in Tokyo, Japan. As of 2020, it operates in 23 countries with over 130 million customers. In the United States, it is not a primary credit card network but has an association with the Discover Network to enable use of JCB cards." ;
	.

fibo-loan-spc-crd:MagneticStripeVerificationCodeValue
	a owl:Class ;
	rdfs:subClassOf fibo-loan-spc-crd:CardVerificationCodeValue ;
	rdfs:label "magnetic stripe verification code or value" ;
	rdfs:isDefinedBy <https://spec.edmcouncil.org/fibo/ontology/LOAN/LoansSpecific/CardAccounts/> ;
	skos:definition "card verification code on a card's magnetic stripe that uses secure cryptographic processes to protect data integrity on the stripe, and reveals any alteration or counterfeiting" ;
	cmns-av:adaptedFrom "https://www.pcisecuritystandards.org/pci_security/glossary"^^xsd:anyURI ;
	.

fibo-loan-spc-crd:MastercardNetwork
	a
		owl:NamedIndividual ,
		fibo-loan-spc-crd:CreditCardNetwork
		;
	rdfs:label "Mastercard network" ;
	rdfs:isDefinedBy <https://spec.edmcouncil.org/fibo/ontology/LOAN/LoansSpecific/CardAccounts/> ;
	skos:definition "credit card network that has its own suite of card protections and benefits, such as identity theft protection and extended warranties" ;
	.

fibo-loan-spc-crd:PaymentCard
	a owl:Class ;
	rdfs:subClassOf
		cmns-doc:LegalDocument ,
		[
			a owl:Restriction ;
			owl:onProperty fibo-fnd-arr-doc:hasExpirationDate ;
			owl:onClass fibo-loan-spc-crd:CardExpirationDate ;
			owl:qualifiedCardinality "1"^^xsd:nonNegativeInteger ;
		] ,
		[
			a owl:Restriction ;
			owl:onProperty fibo-loan-spc-crd:hasCardVerificationCode ;
			owl:onClass fibo-loan-spc-crd:CardVerificationCodeValue ;
			owl:qualifiedCardinality "1"^^xsd:nonNegativeInteger ;
		] ,
		[
			a owl:Restriction ;
			owl:onProperty fibo-loan-spc-crd:hasPrimaryAccountNumber ;
			owl:onClass fibo-loan-spc-crd:PrimaryCardAccountNumber ;
			owl:qualifiedCardinality "1"^^xsd:nonNegativeInteger ;
		] ,
		[
			a owl:Restriction ;
			owl:onProperty fibo-fnd-agr-ctr:isEvidenceFor ;
			owl:someValuesFrom fibo-loan-spc-crd:CardAccount ;
		]
		;
	rdfs:label "payment card" ;
	rdfs:isDefinedBy <https://spec.edmcouncil.org/fibo/ontology/LOAN/LoansSpecific/CardAccounts/> ;
	rdfs:seeAlso <https://www.irs.gov/payments/payment-card-transactions-faqs> ;
	skos:definition "legal document issued by a financial services provider that enables the cardholder to access the funds in the customer's designated bank accounts, or through a credit account and make payments by electronic funds transfer and access automated teller machines (ATMs)" ;
	cmns-av:explanatoryNote
		"For purposes of Payment Card Industry Data Security Standard (PCI DSS), a payment card is any payment card/device that bears the logo of the founding members of PCI SSC, which are American Express, Discover Financial Services, JCB International, MasterCard, or Visa, Inc." ,
		"The term payment card includes credit cards, debit cards, and stored-value cards, as well as payment through any distinctive marks of a payment card (such as a credit card number). A payment card is issued under an agreement that provides standards and mechanisms for settling the transactions between a merchant acquiring bank or similar entity and the providers who accept the cards as payment."
		;
	.

fibo-loan-spc-crd:PaymentCardAgreement
	a owl:Class ;
	rdfs:subClassOf
		fibo-fbc-dae-dbt:CreditAgreement ,
		fibo-fbc-pas-caa:AccountSpecificServiceAgreement ,
		[
			a owl:Restriction ;
			owl:onProperty fibo-fnd-agr-ctr:hasContractParty ;
			owl:someValuesFrom fibo-loan-spc-crd:Cardholder ;
		] ,
		[
			a owl:Restriction ;
			owl:onProperty fibo-fnd-agr-ctr:hasContractParty ;
			owl:someValuesFrom fibo-loan-spc-crd:IssuingFinancialInstitution ;
		] ,
		[
			a owl:Restriction ;
			owl:onProperty fibo-fnd-agr-ctr:isEvidencedBy ;
			owl:someValuesFrom fibo-loan-spc-crd:PaymentCard ;
		] ,
		[
			a owl:Restriction ;
			owl:onProperty cmns-cxtdsg:appliesTo ;
			owl:someValuesFrom fibo-loan-spc-crd:CardAccount ;
		]
		;
	rdfs:label "payment card agreement" ;
	rdfs:isDefinedBy <https://spec.edmcouncil.org/fibo/ontology/LOAN/LoansSpecific/CardAccounts/> ;
	skos:definition "account-specific credit agreement that specifies the terms and conditions under which the payment card is offered to the cardholder by the issuer" ;
	.

fibo-loan-spc-crd:PrimaryCardAccountNumber
	a owl:Class ;
	rdfs:subClassOf
		fibo-fbc-pas-caa:AccountIdentifier ,
		[
			a owl:Restriction ;
			owl:onProperty cmns-id:identifies ;
			owl:onClass fibo-loan-spc-crd:CardAccount ;
			owl:qualifiedCardinality "1"^^xsd:nonNegativeInteger ;
		]
		;
	rdfs:label "primary card account number" ;
	rdfs:isDefinedBy <https://spec.edmcouncil.org/fibo/ontology/LOAN/LoansSpecific/CardAccounts/> ;
	skos:definition "composite identifier of 14 or 16 digits embossed on a bank or payment card and encoded in the card's magnetic strip" ;
	cmns-av:abbreviation "PAN" ;
	cmns-av:explanatoryNote "The PAN identifies the issuer of the card and the account including part of the account number, and contains a check digit that verifies the authenticity of the embossed account number." ;
	cmns-av:synonym "primary account number" ;
	.

fibo-loan-spc-crd:SmartCard
	a owl:Class ;
	rdfs:subClassOf fibo-loan-spc-crd:PaymentCard ;
	rdfs:label "smart card" ;
	rdfs:isDefinedBy <https://spec.edmcouncil.org/fibo/ontology/LOAN/LoansSpecific/CardAccounts/> ;
	skos:definition "payment card that has integrated circuits embedded within it" ;
	cmns-av:adaptedFrom "https://www.pcisecuritystandards.org/pci_security/glossary"^^xsd:anyURI ;
	cmns-av:explanatoryNote "The circuits, also referred to as the 'chip,' contain payment card data including but not limited to data equivalent to the magnetic-stripe data." ;
	.

fibo-loan-spc-crd:ThreeDigitVerificationCodeValue
	a owl:Class ;
	rdfs:subClassOf fibo-loan-spc-crd:CardVerificationCodeValue ;
	rdfs:label "three-digit verification code or value" ;
	rdfs:isDefinedBy <https://spec.edmcouncil.org/fibo/ontology/LOAN/LoansSpecific/CardAccounts/> ;
	skos:definition "card verification code that is the rightmost three-digit value printed in the signature panel area on the back of the card" ;
	cmns-av:adaptedFrom "https://www.pcisecuritystandards.org/pci_security/glossary"^^xsd:anyURI ;
	.

fibo-loan-spc-crd:VisaNetwork
	a
		owl:NamedIndividual ,
		fibo-loan-spc-crd:CreditCardNetwork
		;
	rdfs:label "Visa network" ;
	rdfs:isDefinedBy <https://spec.edmcouncil.org/fibo/ontology/LOAN/LoansSpecific/CardAccounts/> ;
	skos:definition "credit card network that oversees the Visa Signature benefits associated with certain credit cards, such as premium rental car privileges and hotel perks" ;
	.

fibo-loan-spc-crd:hasCardVerificationCode
	a owl:ObjectProperty ;
	rdfs:label "has card verification code" ;
	rdfs:domain fibo-loan-spc-crd:PaymentCard ;
	rdfs:isDefinedBy <https://spec.edmcouncil.org/fibo/ontology/LOAN/LoansSpecific/CardAccounts/> ;
	rdfs:range fibo-loan-spc-crd:CardVerificationCodeValue ;
	skos:definition "links a credit card to either: (1) magnetic-stripe data, or (2) printed security features that are used to protect data integrity and limit alteration, counterfeiting and fraud generally" ;
	.

fibo-loan-spc-crd:hasCreditCardNetwork
	a owl:ObjectProperty ;
	rdfs:subPropertyOf cmns-cls:isClassifiedBy ;
	rdfs:label "has credit card network" ;
	rdfs:isDefinedBy <https://spec.edmcouncil.org/fibo/ontology/LOAN/LoansSpecific/CardAccounts/> ;
	rdfs:range fibo-loan-spc-crd:CreditCardNetwork ;
	skos:definition "indicates the underlying network for credit card product" ;
	.

fibo-loan-spc-crd:hasPrimaryAccountNumber
	a owl:ObjectProperty ;
	rdfs:label "has primary account number" ;
	rdfs:domain fibo-loan-spc-crd:PaymentCard ;
	rdfs:isDefinedBy <https://spec.edmcouncil.org/fibo/ontology/LOAN/LoansSpecific/CardAccounts/> ;
	rdfs:range fibo-loan-spc-crd:PrimaryCardAccountNumber ;
	skos:definition "specifies the account number displayed on the face of the card" ;
	skos:editorialNote "modeled independently of 'identifies' in order to circumvent circular reasoning challenges" ;
	.

fibo-loan-spc-crd:usesCurrency
	a owl:ObjectProperty ;
	rdfs:subPropertyOf cmns-cxtdsg:uses ;
	rdfs:label "uses currency" ;
	rdfs:isDefinedBy <https://spec.edmcouncil.org/fibo/ontology/LOAN/LoansSpecific/CardAccounts/> ;
	rdfs:range fibo-fnd-acc-cur:Currency ;
	skos:definition "indicates the currency defined for the credit card product" ;
	.

