# baseURI: https://spec.edmcouncil.org/fibo/ontology/master/2025Q1/DER/SecurityBasedDerivatives/SecurityBasedDerivatives/
# imports: https://spec.edmcouncil.org/fibo/ontology/master/2025Q1/DER/DerivativesContracts/DerivativesBasics/
# imports: https://spec.edmcouncil.org/fibo/ontology/master/2025Q1/DER/DerivativesContracts/Swaps/
# imports: https://spec.edmcouncil.org/fibo/ontology/master/2025Q1/FBC/DebtAndEquities/Debt/
# imports: https://spec.edmcouncil.org/fibo/ontology/master/2025Q1/FBC/FinancialInstruments/FinancialInstruments/
# imports: https://spec.edmcouncil.org/fibo/ontology/master/2025Q1/FBC/ProductsAndServices/FinancialProductsAndServices/
# imports: https://spec.edmcouncil.org/fibo/ontology/master/2025Q1/FND/Utilities/AnnotationVocabulary/
# imports: https://spec.edmcouncil.org/fibo/ontology/master/2025Q1/IND/Indicators/Indicators/
# imports: https://spec.edmcouncil.org/fibo/ontology/master/2025Q1/IND/MarketIndices/BasketIndices/
# imports: https://spec.edmcouncil.org/fibo/ontology/master/2025Q1/SEC/Debt/DebtInstruments/
# imports: https://spec.edmcouncil.org/fibo/ontology/master/2025Q1/SEC/Equities/EquityInstruments/
# imports: https://spec.edmcouncil.org/fibo/ontology/master/2025Q1/SEC/Securities/Baskets/
# imports: https://www.omg.org/spec/Commons/AnnotationVocabulary/
# imports: https://www.omg.org/spec/Commons/Collections/
# imports: https://www.omg.org/spec/Commons/RolesAndCompositions/

@base <https://spec.edmcouncil.org/fibo/ontology/master/2025Q1/DER/SecurityBasedDerivatives/SecurityBasedDerivatives/> .
@prefix cmns-av: <https://www.omg.org/spec/Commons/AnnotationVocabulary/> .
@prefix cmns-col: <https://www.omg.org/spec/Commons/Collections/> .
@prefix cmns-rlcmp: <https://www.omg.org/spec/Commons/RolesAndCompositions/> .
@prefix dcterms: <http://purl.org/dc/terms/> .
@prefix fibo-der-sbd-sbd: <https://spec.edmcouncil.org/fibo/ontology/DER/SecurityBasedDerivatives/SecurityBasedDerivatives/> .
@prefix fibo-fbc-dae-dbt: <https://spec.edmcouncil.org/fibo/ontology/FBC/DebtAndEquities/Debt/> .
@prefix fibo-fbc-fi-fi: <https://spec.edmcouncil.org/fibo/ontology/FBC/FinancialInstruments/FinancialInstruments/> .
@prefix fibo-fnd-utl-av: <https://spec.edmcouncil.org/fibo/ontology/FND/Utilities/AnnotationVocabulary/> .
@prefix fibo-ind-mkt-bas: <https://spec.edmcouncil.org/fibo/ontology/IND/MarketIndices/BasketIndices/> .
@prefix fibo-sec-dbt-dbti: <https://spec.edmcouncil.org/fibo/ontology/SEC/Debt/DebtInstruments/> .
@prefix fibo-sec-sec-bsk: <https://spec.edmcouncil.org/fibo/ontology/SEC/Securities/Baskets/> .
@prefix owl: <http://www.w3.org/2002/07/owl#> .
@prefix rdf: <http://www.w3.org/1999/02/22-rdf-syntax-ns#> .
@prefix rdfs: <http://www.w3.org/2000/01/rdf-schema#> .
@prefix skos: <http://www.w3.org/2004/02/skos/core#> .
@prefix xsd: <http://www.w3.org/2001/XMLSchema#> .

<https://spec.edmcouncil.org/fibo/ontology/DER/SecurityBasedDerivatives/SecurityBasedDerivatives/>
	a owl:Ontology ;
	rdfs:label "Security-Based Derivatives Ontology" ;
	dcterms:abstract "This ontology defines common concepts for derivatives based on securities as their underliers, including those based on indices or baskets of these assets." ;
	dcterms:license """Copyright (c) 2016-2025 EDM Council, Inc.
Copyright (c) 2016-2025 Object Management Group, Inc.

Permission is hereby granted, free of charge, to any person obtaining a copy of this software and associated documentation files (the 'Software'), to deal in the Software without restriction, including without limitation the rights to use, copy, modify, merge, publish, distribute, sublicense, and/or sell copies of the Software, and to permit persons to whom the Software is furnished to do so, subject to the following conditions:

The above copyright notice and this permission notice shall be included in all copies or substantial portions of the Software.

THE SOFTWARE IS PROVIDED 'AS IS', WITHOUT WARRANTY OF ANY KIND, EXPRESS OR IMPLIED, INCLUDING BUT NOT LIMITED TO THE WARRANTIES OF MERCHANTABILITY, FITNESS FOR A PARTICULAR PURPOSE AND NONINFRINGEMENT. IN NO EVENT SHALL THE AUTHORS OR COPYRIGHT HOLDERS BE LIABLE FOR ANY CLAIM, DAMAGES OR OTHER LIABILITY, WHETHER IN AN ACTION OF CONTRACT, TORT OR OTHERWISE, ARISING FROM, OUT OF OR IN CONNECTION WITH THE SOFTWARE OR THE USE OR OTHER DEALINGS IN THE SOFTWARE.
		
See https://opensource.org/licenses/MIT.""" ;
	owl:imports
		<https://spec.edmcouncil.org/fibo/ontology/master/2025Q1/DER/DerivativesContracts/DerivativesBasics/> ,
		<https://spec.edmcouncil.org/fibo/ontology/master/2025Q1/DER/DerivativesContracts/Swaps/> ,
		<https://spec.edmcouncil.org/fibo/ontology/master/2025Q1/FBC/DebtAndEquities/Debt/> ,
		<https://spec.edmcouncil.org/fibo/ontology/master/2025Q1/FBC/FinancialInstruments/FinancialInstruments/> ,
		<https://spec.edmcouncil.org/fibo/ontology/master/2025Q1/FBC/ProductsAndServices/FinancialProductsAndServices/> ,
		<https://spec.edmcouncil.org/fibo/ontology/master/2025Q1/FND/Utilities/AnnotationVocabulary/> ,
		<https://spec.edmcouncil.org/fibo/ontology/master/2025Q1/IND/Indicators/Indicators/> ,
		<https://spec.edmcouncil.org/fibo/ontology/master/2025Q1/IND/MarketIndices/BasketIndices/> ,
		<https://spec.edmcouncil.org/fibo/ontology/master/2025Q1/SEC/Debt/DebtInstruments/> ,
		<https://spec.edmcouncil.org/fibo/ontology/master/2025Q1/SEC/Equities/EquityInstruments/> ,
		<https://spec.edmcouncil.org/fibo/ontology/master/2025Q1/SEC/Securities/Baskets/> ,
		<https://www.omg.org/spec/Commons/AnnotationVocabulary/> ,
		<https://www.omg.org/spec/Commons/Collections/> ,
		<https://www.omg.org/spec/Commons/RolesAndCompositions/>
		;
	owl:versionIRI <https://spec.edmcouncil.org/fibo/ontology/master/2025Q1/DER/SecurityBasedDerivatives/SecurityBasedDerivatives/> ;
	skos:changeNote
		"The https://spec.edmcouncil.org/fibo/ontology/DER/SecurityBasedDerivatives/SecurityBasedDerivatives.rdf version of this ontology was modified to augment the concept of a basket of debt instruments with several variants (SEC-181)." ,
		"The https://spec.edmcouncil.org/fibo/ontology/DER/SecurityBasedDerivatives/SecurityBasedDerivatives.rdf version of this ontology was modified to replace content that is now available in the OMG Commons Ontology Library (Commons) v1.1 (FND-380)." ,
		"The https://spec.edmcouncil.org/fibo/ontology/DER/SecurityBasedDerivatives/SecurityBasedDerivatives.rdf version of this ontology was modified to simplify and refine definitions related to underliers (DER-112)." ,
		"The https://spec.edmcouncil.org/fibo/ontology/DER/SecurityBasedDerivatives/SecurityBasedDerivatives.rdf version of this ontology was modified to use the Commons Ontology Library (Commons) Annotation Vocabulary rather than the OMG's Specification Metadata vocabulary, to move the definition of an underlier and the related property, has underlier, to financial instruments so that these concepts are also available for use in relation to pool-backed securities." ,
		"The https://spec.edmcouncil.org/fibo/ontology/DER/SecurityBasedDerivatives/SecurityBasedDerivatives.rdf version of this ontology was modified to use the Commons Ontology Library (Commons) rather than the OMG's Languages, Countries and Codes (LCC), eliminating redundancies in FIBO as appropriate."
		;
	fibo-fnd-utl-av:hasMaturityLevel fibo-fnd-utl-av:Release ;
	cmns-av:copyright
		"Copyright (c) 2016-2025 EDM Council, Inc." ,
		"Copyright (c) 2016-2025 Object Management Group, Inc."
		;
	.

fibo-der-sbd-sbd:BasketOfDebtInstruments
	a owl:Class ;
	rdfs:subClassOf
		fibo-sec-sec-bsk:BasketOfSecurities ,
		[
			a owl:Restriction ;
			owl:onProperty cmns-col:hasConstituent ;
			owl:someValuesFrom [
				a owl:Restriction ;
				owl:onProperty cmns-col:comprises ;
				owl:allValuesFrom fibo-fbc-fi-fi:DebtInstrument ;
			] ;
		]
		;
	rdfs:label "basket of debt instruments"@en ;
	rdfs:isDefinedBy <https://spec.edmcouncil.org/fibo/ontology/DER/SecurityBasedDerivatives/SecurityBasedDerivatives/> ;
	skos:definition "basket of securities whose constituents are debt instruments"@en ;
	.

fibo-der-sbd-sbd:CapitalizedLeaseObligationDebtBasket
	a owl:Class ;
	rdfs:subClassOf
		fibo-der-sbd-sbd:BasketOfDebtInstruments ,
		[
			a owl:Restriction ;
			owl:onProperty cmns-col:hasConstituent ;
			owl:someValuesFrom [
				a owl:Restriction ;
				owl:onProperty cmns-col:comprises ;
				owl:allValuesFrom fibo-fbc-dae-dbt:Lease ;
			] ;
		]
		;
	rdfs:label "capitalized lease obligation debt basket"@en ;
	rdfs:isDefinedBy <https://spec.edmcouncil.org/fibo/ontology/DER/SecurityBasedDerivatives/SecurityBasedDerivatives/> ;
	skos:definition "basket of debt instruments whose constituents are contracts entitling a renter the temporary use of an asset and, in accounting terms, has asset ownership characteristics"@en ;
	cmns-av:explanatoryNote "A capitalized lease obligation basket is increasingly broadly drafted to include indebtedness incurred to finance the purchase, improvement, repair, renewal etc. of property (including the purchase of stock of a person owning such property)."@en ;
	.

fibo-der-sbd-sbd:ContributionDebtBasket
	a owl:Class ;
	rdfs:subClassOf fibo-der-sbd-sbd:BasketOfDebtInstruments ;
	rdfs:label "contribution debt basket"@en ;
	rdfs:isDefinedBy <https://spec.edmcouncil.org/fibo/ontology/DER/SecurityBasedDerivatives/SecurityBasedDerivatives/> ;
	skos:definition "basket of debt instruments that allows a company to incur an amount of indebtedness that is equal to (or in top tier sponsor transactions in the U.S., up to two times) the amount of equity contributed to the group"@en ;
	cmns-av:explanatoryNote
		"A non-guarantor debt basket is often also permitted to be secured by assets of a subsidiary other than the issuer/borrower or guarantors."@en ,
		"In U.S. law, a non-guarantor debt basket is a shared basket in an amount not to exceed the greater of $150,000,000 and 20% of Consolidated EBITDA for the most recently ended Test Period at any time outstanding that may be used for (A) the incurrence of certain Indebtedness by Restricted Subsidiaries that are not Loan Parties under Sections 6.01(a)(xii), 6.01(a)(xix) and 6.01(a)(xx) and (B) Secured Cash Management Obligations of any Restricted Subsidiary that is not a Loan Party."@en
		;
	.

fibo-der-sbd-sbd:CreditFacilityDebtBasket
	a owl:Class ;
	rdfs:subClassOf
		fibo-der-sbd-sbd:BasketOfDebtInstruments ,
		[
			a owl:Restriction ;
			owl:onProperty cmns-col:hasConstituent ;
			owl:someValuesFrom [
				a owl:Restriction ;
				owl:onProperty cmns-col:comprises ;
				owl:allValuesFrom fibo-fbc-dae-dbt:CreditFacility ;
			] ;
		]
		;
	rdfs:label "credit facility debt basket"@en ;
	rdfs:isDefinedBy <https://spec.edmcouncil.org/fibo/ontology/DER/SecurityBasedDerivatives/SecurityBasedDerivatives/> ;
	skos:definition "basket of securities whose constituents are credit agreements that allow the borrower to periodically take out money over an extended period of time rather than reapplying for a loan every time they need funds"@en ;
	cmns-av:explanatoryNote "The credit facility debt basket consists of a number of credit facilities including revolving loans/line of credit, committed facilities, letters of credit and most retail credit accounts. The first port of call for issuers is the credit facility debt basket. In addition to the fixed dollar (or euro) amounts, credit facility debt baskets in senior secured notes and indentures typically provide for a grower component that is the greater of the fixed dollar/euro amount and a percentage of total assets, total tangible assets or EBITDA."@en ;
	.

fibo-der-sbd-sbd:DebtInstrumentDerivative
	a owl:Class ;
	rdfs:subClassOf
		fibo-der-sbd-sbd:SecurityBasedDerivative ,
		[
			a owl:Restriction ;
			owl:onProperty fibo-fbc-fi-fi:hasUnderlier ;
			owl:someValuesFrom [
				a owl:Restriction ;
				owl:onProperty cmns-rlcmp:isPlayedBy ;
				owl:someValuesFrom [
					a owl:Class ;
					owl:unionOf (
						fibo-der-sbd-sbd:BasketOfDebtInstruments
						fibo-sec-dbt-dbti:TradableDebtInstrument
						fibo-ind-mkt-bas:CreditIndex
						fibo-ind-mkt-bas:BasketOfCreditRisks
					) ;
				] ;
			] ;
		]
		;
	rdfs:label "debt instrument derivative" ;
	rdfs:isDefinedBy <https://spec.edmcouncil.org/fibo/ontology/DER/SecurityBasedDerivatives/SecurityBasedDerivatives/> ;
	skos:definition "security-based derivative whose underlier is a debt observable" ;
	.

fibo-der-sbd-sbd:DebtObservable
	a owl:Class ;
	rdfs:isDefinedBy <https://spec.edmcouncil.org/fibo/ontology/DER/SecurityBasedDerivatives/SecurityBasedDerivatives/> ;
	owl:deprecated "true"^^xsd:boolean ;
	owl:equivalentClass fibo-fbc-fi-fi:Underlier ;
	.

fibo-der-sbd-sbd:EquityDerivative
	a owl:Class ;
	rdfs:subClassOf
		fibo-der-sbd-sbd:SecurityBasedDerivative ,
		[
			a owl:Restriction ;
			owl:onProperty fibo-fbc-fi-fi:hasUnderlier ;
			owl:someValuesFrom [
				a owl:Restriction ;
				owl:onProperty cmns-rlcmp:isPlayedBy ;
				owl:someValuesFrom [
					a owl:Class ;
					owl:unionOf (
						fibo-ind-mkt-bas:BasketOfEquities
						fibo-fbc-fi-fi:EquityInstrument
						fibo-ind-mkt-bas:EquityIndex
					) ;
				] ;
			] ;
		]
		;
	rdfs:label "equity derivative" ;
	rdfs:isDefinedBy <https://spec.edmcouncil.org/fibo/ontology/DER/SecurityBasedDerivatives/SecurityBasedDerivatives/> ;
	skos:definition "security-based derivative whose underlier is based on equities (e.g. shares, basket of equities or index) or their cashflow(s)" ;
	.

fibo-der-sbd-sbd:EquityObservable
	a owl:Class ;
	rdfs:isDefinedBy <https://spec.edmcouncil.org/fibo/ontology/DER/SecurityBasedDerivatives/SecurityBasedDerivatives/> ;
	owl:deprecated "true"^^xsd:boolean ;
	owl:equivalentClass fibo-fbc-fi-fi:Underlier ;
	.

fibo-der-sbd-sbd:GeneralDebtBasket
	a owl:Class ;
	rdfs:subClassOf fibo-der-sbd-sbd:BasketOfDebtInstruments ;
	rdfs:label "general debt basket"@en ;
	rdfs:isDefinedBy <https://spec.edmcouncil.org/fibo/ontology/DER/SecurityBasedDerivatives/SecurityBasedDerivatives/> ;
	skos:definition "basket of debt instruments that provides additional capacity for potential funding and does not require the proceeds to be used for any particular purpose"@en ;
	cmns-av:explanatoryNote "The general debt basket has increasingly become a basket for additional secured debt. Lenders providing funding to companies need to carefully consider whether any previous debt incurred by the company using this basket has reduced the available capacity."@en ;
	.

fibo-der-sbd-sbd:IncrementalFacilityDebtBasket
	a owl:Class ;
	rdfs:subClassOf fibo-der-sbd-sbd:CreditFacilityDebtBasket ;
	rdfs:label "incremental facility debt basket"@en ;
	rdfs:isDefinedBy <https://spec.edmcouncil.org/fibo/ontology/DER/SecurityBasedDerivatives/SecurityBasedDerivatives/> ;
	skos:definition "basket of credit facilities whose constituents are extensible, allowing companies to borrow an additional term loan or revolving credit facility (or increase the commitments applicable thereto) under the same credit agreement subject to certain parameters"@en ;
	cmns-av:explanatoryNote "The incremental debt basket is available to borrowers and guarantors only; it cannot be used by non-guarantor entities to raise indebtedness. The size of the incremental debt basket varies depending on the size and creditworthiness of the credit group. The principle of a basket consists of allowing the borrower, up to a maximum determined amount, to make restricted payments, disposals or investments, or take on incremental debt. Commonly, a basket is expressed as subject to restrictions based on a fixed ('hard cap') amount (e.g., may not exceed EUR 5,000,000)."@en ;
	cmns-av:synonym "builder basket"@en ;
	.

fibo-der-sbd-sbd:LocalLinesOfCreditDebtBasket
	a owl:Class ;
	rdfs:subClassOf
		fibo-der-sbd-sbd:BasketOfDebtInstruments ,
		[
			a owl:Restriction ;
			owl:onProperty cmns-col:hasConstituent ;
			owl:someValuesFrom [
				a owl:Restriction ;
				owl:onProperty cmns-col:comprises ;
				owl:allValuesFrom fibo-fbc-dae-dbt:RevolvingLineOfCredit ;
			] ;
		]
		;
	rdfs:label "local lines of credit debt basket"@en ;
	rdfs:isDefinedBy <https://spec.edmcouncil.org/fibo/ontology/DER/SecurityBasedDerivatives/SecurityBasedDerivatives/> ;
	skos:definition "basket of debt instruments that may be relevant for companies with international operations, often permitting debt to be incurred by a non-guarantor restricted subsidiary"@en ;
	.

fibo-der-sbd-sbd:Non-GuarantorDebtBasket
	a owl:Class ;
	rdfs:subClassOf fibo-der-sbd-sbd:BasketOfDebtInstruments ;
	rdfs:label "non-guarantor debt basket"@en ;
	rdfs:isDefinedBy <https://spec.edmcouncil.org/fibo/ontology/DER/SecurityBasedDerivatives/SecurityBasedDerivatives/> ;
	skos:definition "basket of debt instruments that include a provision allowing certain subsidiaries within a corporate group, which are not part of the loan guarantee, to incur a specified amount of indebtedness"@en ;
	cmns-av:explanatoryNote
		"A non-guarantor debt basket is often also permitted to be secured by assets of a subsidiary other than the issuer/borrower or guarantors."@en ,
		"In U.S. law, a non-guarantor debt basket is a shared basket in an amount not to exceed the greater of $150,000,000 and 20% of Consolidated EBITDA for the most recently ended Test Period at any time outstanding that may be used for (A) the incurrence of certain Indebtedness by Restricted Subsidiaries that are not Loan Parties under Sections 6.01(a)(xii), 6.01(a)(xix) and 6.01(a)(xx) and (B) Secured Cash Management Obligations of any Restricted Subsidiary that is not a Loan Party."@en
		;
	.

fibo-der-sbd-sbd:RatioDebtBasket
	a owl:Class ;
	rdfs:subClassOf fibo-der-sbd-sbd:BasketOfDebtInstruments ;
	rdfs:label "ratio debt basket"@en ;
	rdfs:isDefinedBy <https://spec.edmcouncil.org/fibo/ontology/DER/SecurityBasedDerivatives/SecurityBasedDerivatives/> ;
	skos:definition "basket of debt instruments whose constituents are specified based on a leverage ratio based on total debt rather than only secured debt"@en ;
	cmns-av:explanatoryNote "The ratio basket provides different ratio tests depending on the type of indebtedness being incurred (for example, first lien leverage ratio in respect of first lien indebtedness, senior secured leverage ratio in respect of indebtedness secured by a junior lien and a total net leverage ratio or interest coverage ratio in respect of unsecured indebtedness). A ratio basket would typically allow the borrower to incur debt secured on a senior secured basis subject to a maximum senior secured leverage ratio and unsecured debt subject to a maximum total leverage ratio."@en ;
	.

fibo-der-sbd-sbd:SecurityBasedDerivative
	a owl:Class ;
	rdfs:subClassOf
		fibo-fbc-fi-fi:DerivativeInstrument ,
		[
			a owl:Restriction ;
			owl:onProperty fibo-fbc-fi-fi:hasUnderlier ;
			owl:someValuesFrom [
				a owl:Restriction ;
				owl:onProperty cmns-rlcmp:isPlayedBy ;
				owl:someValuesFrom [
					a owl:Class ;
					owl:unionOf (
						fibo-sec-sec-bsk:BasketOfSecurities
						fibo-fbc-fi-fi:Security
						fibo-ind-mkt-bas:ReferenceIndex
					) ;
				] ;
			] ;
		]
		;
	rdfs:label "security-based derivative"@en ;
	rdfs:isDefinedBy <https://spec.edmcouncil.org/fibo/ontology/DER/SecurityBasedDerivatives/SecurityBasedDerivatives/> ;
	skos:definition "derivative instrument whose underlier is based on a security, including collections of securities and indices based on securities" ;
	.

fibo-der-sbd-sbd:SecurityUnderlier
	a owl:Class ;
	rdfs:isDefinedBy <https://spec.edmcouncil.org/fibo/ontology/DER/SecurityBasedDerivatives/SecurityBasedDerivatives/> ;
	owl:deprecated "true"^^xsd:boolean ;
	owl:equivalentClass fibo-fbc-fi-fi:Underlier ;
	.

